some restructuring + small proofs

cedar-lean/Cedar/Thm/Soundness.lean
@@ -15,81 +15,17 @@
 -/
 
 import Cedar.Spec
-import Cedar.Thm.Lemmas.Typechecker
+import Cedar.Thm.Lemmas.Validator
 import Mathlib.Data.List.Basic
 
 /-!
 This file defines the top-level soundness property for the valdator.
-
-todo: fill in `sorry`s. Some invariants may need to be adjusted. The current
-definitions are an informed guess based on the corresponding Dafny proof.
 --/
 
 namespace Cedar.Thm
 
 open Cedar.Spec
 open Cedar.Validation
-
-def EvaluatesToBool (policy : Policy) (request : Request) (entities : Entities) : Prop :=
-  ∃ (b : Bool), EvaluatesTo policy.toExpr request entities b
-
-/--
-If a policy successfully validates, then evaluating that policy with any request
-will either (1) return a Boolean value or (2) return an error of type `entityDoesNotExist`
-or `extensionError`. Both options are encoded in the `EvaluatesToBool` predicate.
-The validator cannot protect against `entityDoesNotExist` and `extensionError`
-errors because it has no knowledge of the entities/context that will be provided
-at authorization time.
--/
-theorem typecheck_policy_is_sound (policy : Policy) (env : Environment) (t : CedarType) (request : Request) (entities : Entities) :
-  RequestAndEntitiesMatchEnvironment env request entities →
-  typecheckPolicy policy env = .ok t →
-  EvaluatesToBool policy request entities
-:= by
-  intro h₀ h₁
-  unfold typecheckPolicy at h₁
-  cases h₂ : (typeOf (Policy.toExpr policy) ∅ env) <;>
-  rw [h₂] at h₁ <;>
-  simp at h₁
-  case ok res =>
-    cases h₃ : (res.fst ⊑ CedarType.bool BoolType.anyBool) <;>
-    rw [h₃] at h₁ <;>
-    simp at h₁
-    clear h₁ t
-    have h₁ : GuardedCapabilitiesInvariant policy.toExpr res.2 request entities ∧ ∃ (v : Value), EvaluatesTo policy.toExpr request entities v ∧ InstanceOfType v res.1 := by
-      apply type_of_is_sound (env:=env) (c₁:=∅)
-      apply empty_capabilities_invariant
-      apply h₀
-      apply h₂
-    cases h₁ with
-    | intro _ h₁ =>
-      cases h₁ with
-      | intro v h₁ =>
-        cases h₁ with
-        | intro h₁ h₄ =>
-          have h₅ : ∃ b, v = .prim (.bool b) := by
-            apply instance_of_type_bool_is_bool
-            apply h₄
-            apply h₃
-          cases h₅ with
-          | intro b h₅ =>
-            unfold EvaluatesToBool
-            exists b
-            rewrite [← h₅]
-            apply h₁
-
-def RequestMatchesSchema (schema : Schema) (request : Request) : Prop :=
-  match schema.acts.find? request.action with
-  | some entry =>
-      request.principal.ty ∈ entry.appliesToPricipal ∧
-      request.resource.ty ∈ entry.appliesToResource ∧
-      InstanceOfType request.context (.record entry.context)
-  | _ => False
-
-def RequestAndEntitiesMatchSchema (schema : Schema) (request : Request) (entities : Entities) : Prop :=
-  RequestMatchesSchema schema request ∧
-  InstanceOfEntityTypeStore entities schema.ets ∧
-  InstanceOfActionStore entities (schema.acts.mapOnValues (fun entry => entry.descendants))
 
 /--
 Top-level soundness theorem: If validation succeeds, then for any request
@@ -100,4 +36,13 @@ theorem validate_is_sound (policies : Policies) (schema : Schema) (request : Req
   validate policies schema = .ok () →
   ∀ policy, policy ∈ policies → EvaluatesToBool policy request entities
 := by
-  sorry
+  intro h₀ h₁ policy hₚ
+  unfold validate at h₁
+  simp at h₁
+  apply typecheck_policy_with_environments_is_sound (envs:=schema.toEnvironments)
+  intro env hₑ
+  apply match_schema_implies_match_environments (schema:=schema)
+  apply h₀
+  apply hₑ
+  apply (forM_all_ok _ _ h₁)
+  assumption
