cedar-lean/Cedar/Thm/Lemmas/Validator.lean
@@ -1,0 +1,131 @@
+/-
+ Copyright 2022-2023 Amazon.com, Inc. or its affiliates. All Rights Reserved.
+
+ Licensed under the Apache License, Version 2.0 (the "License");
+ you may not use this file except in compliance with the License.
+ You may obtain a copy of the License at
+
+      https://www.apache.org/licenses/LICENSE-2.0
+
+ Unless required by applicable law or agreed to in writing, software
+ distributed under the License is distributed on an "AS IS" BASIS,
+ WITHOUT WARRANTIES OR CONDITIONS OF ANY KIND, either express or implied.
+ See the License for the specific language governing permissions and
+ limitations under the License.
+-/
+
+import Cedar.Spec
+import Cedar.Validation
+import Cedar.Thm.Lemmas.Typechecker
+
+/-!
+This file contains useful definitions and lemmas about the `Validator` functions.
+
+todo: fill in `sorry`s. Some invariants may need to be adjusted. The current
+definitions are an informed guess based on the corresponding Dafny proof.
+-/
+
+namespace Cedar.Thm
+
+open Cedar.Data
+open Cedar.Spec
+open Cedar.Validation
+
+def EvaluatesToBool (policy : Policy) (request : Request) (entities : Entities) : Prop :=
+  ∃ (b : Bool), EvaluatesTo policy.toExpr request entities b
+
+/--
+If a policy successfully validates, then evaluating that policy with any request
+will either (1) return a Boolean value or (2) return an error of type `entityDoesNotExist`
+or `extensionError`. Both options are encoded in the `EvaluatesToBool` predicate.
+The validator cannot protect against `entityDoesNotExist` and `extensionError`
+errors because it has no knowledge of the entities/context that will be provided
+at authorization time.
+-/
+theorem typecheck_policy_is_sound (policy : Policy) (env : Environment) (t : CedarType) (request : Request) (entities : Entities) :
+  RequestAndEntitiesMatchEnvironment env request entities →
+  typecheckPolicy policy env = .ok t →
+  EvaluatesToBool policy request entities
+:= by
+  intro h₀ h₁
+  unfold typecheckPolicy at h₁
+  cases h₂ : (typeOf (Policy.toExpr policy) ∅ env) <;>
+  rw [h₂] at h₁ <;>
+  simp at h₁
+  case ok res =>
+    cases h₃ : (res.fst ⊑ CedarType.bool BoolType.anyBool) <;>
+    rw [h₃] at h₁ <;>
+    simp at h₁
+    clear h₁ t
+    have h₁ : GuardedCapabilitiesInvariant policy.toExpr res.2 request entities ∧ ∃ (v : Value), EvaluatesTo policy.toExpr request entities v ∧ InstanceOfType v res.1 := by
+      apply type_of_is_sound (env:=env) (c₁:=∅)
+      apply empty_capabilities_invariant
+      apply h₀
+      apply h₂
+    cases h₁ with
+    | intro _ h₁ =>
+      cases h₁ with
+      | intro v h₁ =>
+        cases h₁ with
+        | intro h₁ h₄ =>
+          have h₅ : ∃ b, v = .prim (.bool b) := by
+            apply instance_of_type_bool_is_bool
+            apply h₄
+            apply h₃
+          cases h₅ with
+          | intro b h₅ =>
+            unfold EvaluatesToBool
+            exists b
+            rewrite [← h₅]
+            apply h₁
+
+def RequestMatchesSchema (schema : Schema) (request : Request) : Prop :=
+  match schema.acts.find? request.action with
+  | some entry =>
+      request.principal.ty ∈ entry.appliesToPricipal ∧
+      request.resource.ty ∈ entry.appliesToResource ∧
+      InstanceOfType request.context (.record entry.context)
+  | _ => False
+
+def RequestAndEntitiesMatchSchema (schema : Schema) (request : Request) (entities : Entities) : Prop :=
+  RequestMatchesSchema schema request ∧
+  InstanceOfEntityTypeStore entities schema.ets ∧
+  InstanceOfActionStore entities (schema.acts.mapOnValues (fun entry => entry.descendants))
+
+theorem match_schema_implies_match_environments (schema : Schema) (request : Request) (entities : Entities) :
+  RequestAndEntitiesMatchSchema schema request entities →
+  ∀ env, env ∈ schema.toEnvironments →
+  RequestAndEntitiesMatchEnvironment env request entities
+:= by
+  sorry
+
+theorem typecheck_policy_with_environments_is_sound (policy : Policy) (envs : List Environment) (request : Request) (entities : Entities) :
+  (∀ env, env ∈ envs → RequestAndEntitiesMatchEnvironment env request entities) →
+  typecheckPolicyWithEnvironments policy envs = .ok () →
+  EvaluatesToBool policy request entities
+:= by
+  sorry
+
+theorem forM_all_ok {α ε} (l : List α) (f : α → Except ε Unit) :
+  l.forM f = .ok () →
+  ∀ x, x ∈ l → f x = .ok ()
+:= by
+  intro h₀ x hₓ
+  induction l
+  case nil => cases hₓ
+  case cons hd tl ih =>
+    simp at h₀
+    simp [bind, Except.bind] at h₀
+    cases hₓ
+    -- x == hd
+    case head =>
+      generalize h : f x = fx
+      cases fx <;> rewrite [h] at h₀ <;> simp at h₀
+      case ok =>
+        rfl
+    -- x ∈ tl
+    case tail =>
+      generalize h : f hd = fhd
+      cases fhd <;> rewrite [h] at h₀ <;> simp at h₀
+      case ok =>
+        apply ih <;> assumption
